src/Init/Internal/Order.lean
@@ -3,8 +3,7 @@ Copyright (c) 2024 Lean FRO, LLC. All rights reserved.
 Released under Apache 2.0 license as described in the file LICENSE.
 Authors: Joachim Breitner
 -/
-
 prelude
-
-import Init.Tailrec.Basic
-import Init.Tailrec.Lemmas
+import Init.Internal.Order.Basic
+import Init.Internal.Order.Lemmas
+import Init.Internal.Order.Tactic
