src/Lean/Elab/PreDefinition/Main.lean
@@ -9,7 +9,7 @@ import Lean.Elab.PreDefinition.Basic
 import Lean.Elab.PreDefinition.Structural
 import Lean.Elab.PreDefinition.WF.Main
 import Lean.Elab.PreDefinition.MkInhabitant
-import Lean.Elab.PreDefinition.Tailrec
+import Lean.Elab.PreDefinition.PartialFixpoint
 
 namespace Lean.Elab
 open Meta
@@ -164,7 +164,7 @@ Checks consistency of a clique of TerminationHints:
 
 * If not all have a hint, the hints are ignored (log error)
 * None have both `termination_by` and `nontermination` (throw error)
-* If one has `structural` or `tailrec`, check that all have it (else throw error)
+* If one has `structural` or `partialFixpoint`, check that all have it (else throw error)
 * A `structural` should not have a `decreasing_by` (else log error)
 
 -/
@@ -173,14 +173,14 @@ def checkTerminationByHints (preDefs : Array PreDefinition) : CoreM Unit := do
   let preDefsWithout := preDefs.filter (·.termination.terminationBy?.isNone)
   let structural :=
     preDefWith.termination.terminationBy? matches some {structural := true, ..}
-  let tailrec := preDefWith.termination.tailrec?.isSome
+  let partialFixpoint := preDefWith.termination.partialFixpoint?.isSome
   for preDef in preDefs do
     if let .some termBy := preDef.termination.terminationBy? then
-      if let .some tailrecStx := preDef.termination.tailrec? then
-        throwErrorAt tailrecStx (m!"conflicting annotations: this function cannot be both " ++
+      if let .some partialFixpointStx := preDef.termination.partialFixpoint? then
+        throwErrorAt partialFixpointStx (m!"conflicting annotations: this function cannot be both " ++
           m!"terminating and non-terminating")
 
-      if !structural && !tailrec && !preDefsWithout.isEmpty then
+      if !structural && !partialFixpoint && !preDefsWithout.isEmpty then
         let m := MessageData.andList (preDefsWithout.toList.map (m!"{·.declName}"))
         let doOrDoes := if preDefsWithout.size = 1 then "does" else "do"
         logErrorAt termBy.ref (m!"incomplete set of `termination_by` annotations:\n"++
@@ -201,22 +201,22 @@ def checkTerminationByHints (preDefs : Array PreDefinition) : CoreM Unit := do
           logErrorAt decr.ref (m!"Invalid `decreasing_by`; this function is marked as " ++
             m!"structurally recursive, so no explicit termination proof is needed.")
 
-    if tailrec && preDef.termination.tailrec?.isNone then
+    if partialFixpoint && preDef.termination.partialFixpoint?.isNone then
       throwErrorAt preDef.ref (m!"Invalid `termination_by`; this function is mutually " ++
         m!"recursive with {preDefWith.declName}, which is marked as " ++
-        m!"`nontermination_tailrecursive` so this one also needs to be marked " ++
-        m!"`nontermination_tailrecursive`.")
+        m!"`nontermination_partialFixpointursive` so this one also needs to be marked " ++
+        m!"`nontermination_partialFixpointursive`.")
 
-    if preDef.termination.tailrec?.isSome then
+    if preDef.termination.partialFixpoint?.isSome then
         if let .some decr := preDef.termination.decreasingBy? then
           logErrorAt decr.ref (m!"Invalid `decreasing_by`; this function is marked as " ++
             m!"nonterminating, so no explicit termination proof is needed.")
 
-    if !tailrec then
-      if let some stx := preDef.termination.tailrec? then
+    if !partialFixpoint then
+      if let some stx := preDef.termination.partialFixpoint? then
       throwErrorAt stx (m!"Invalid `termination_by`; this function is mutually " ++
        m!"recursive with {preDefWith.declName}, which is not also marked as " ++
-        m!"`nontermination_tailrecursive`, so this one cannot be either.")
+        m!"`nontermination_partialFixpointursive`, so this one cannot be either.")
 
 /--
 Elaborates the `TerminationHint` in the clique to `TerminationArguments`
@@ -232,9 +232,9 @@ def shouldUseStructural (preDefs : Array PreDefinition) : Bool :=
   preDefs.any fun preDef =>
     preDef.termination.terminationBy? matches some {structural := true, ..}
 
-def shouldUseTailrec (preDefs : Array PreDefinition) : Bool :=
+def shouldUsepartialFixpoint (preDefs : Array PreDefinition) : Bool :=
   preDefs.any fun preDef =>
-    preDef.termination.tailrec?.isSome
+    preDef.termination.partialFixpoint?.isSome
 
 def shouldUseWF (preDefs : Array PreDefinition) : Bool :=
   preDefs.any fun preDef =>
@@ -282,8 +282,8 @@ def addPreDefinitions (preDefs : Array PreDefinition) : TermElabM Unit := withLC
             let termArg?s ← elabTerminationByHints preDefs
             if shouldUseStructural preDefs then
               structuralRecursion preDefs termArg?s
-            else if shouldUseTailrec preDefs then
-              tailRecursion preDefs
+            else if shouldUsepartialFixpoint preDefs then
+              partialFixpoint preDefs
             else if shouldUseWF preDefs then
               wfRecursion preDefs termArg?s
             else
