src/Lean/Elab/PreDefinition/WF/Eqns.lean
@@ -10,11 +10,12 @@ import Lean.Elab.PreDefinition.Basic
 import Lean.Elab.PreDefinition.Eqns
 import Lean.Meta.ArgsPacker.Basic
 import Init.Data.Array.Basic
-import Init.Tailrec
+import Init.Internal.Order.Basic
 
 namespace Lean.Elab.WF
 open Meta
 open Eqns
+open Lean.Internal
 
 structure EqnInfo extends EqnInfoCore where
   declNames       : Array Name
@@ -29,7 +30,7 @@ private partial def deltaLHSUntilFix (mvarId : MVarId) : MetaM MVarId := mvarId.
   let some (_, lhs, _) := target.eq? | throwTacticEx `deltaLHSUntilFix mvarId "equality expected"
   if lhs.isAppOf ``WellFounded.fix then
     return mvarId
-  else if lhs.isAppOf ``Tailrec.fix then
+  else if lhs.isAppOf ``Order.fix then
     return mvarId
   else
     deltaLHSUntilFix (← deltaLHS mvarId)
@@ -40,10 +41,10 @@ private def rwFixEq (mvarId : MVarId) : MetaM MVarId := mvarId.withContext do
   let h ←
     if lhs.isAppOf ``WellFounded.fix then
       pure <| mkAppN (mkConst ``WellFounded.fix_eq lhs.getAppFn.constLevels!) lhs.getAppArgs
-    else if lhs.isAppOf ``Tailrec.fix then
+    else if lhs.isAppOf ``Order.fix then
       let x := lhs.getAppArgs.back!
       let args := lhs.getAppArgs.pop
-      mkAppM ``congrFun #[mkAppN (mkConst ``Tailrec.fix_eq lhs.getAppFn.constLevels!) args, x]
+      mkAppM ``congrFun #[mkAppN (mkConst ``Order.fix_eq lhs.getAppFn.constLevels!) args, x]
     else
       throwTacticEx `rwFixEq mvarId "expected fixed-point application"
   let some (_, _, lhsNew) := (← inferType h).eq? | unreachable!
