tests/lean/run/partial_fixpoint_monotonicity.lean
@@ -1,0 +1,52 @@
+-- Tests the `monotonicity` tactic
+
+-- These can move to Init after a stage0 update
+open Lean.Internal.Order in
+attribute [partial_monotone]
+  monotone_ite
+  monotone_dite
+  monotone_bind
+  monotone_mapM
+  monotone_mapFinIdxM
+
+
+/-
+Shoudl test that the tactic syntax is scoped, but cannot use #guard_msgs to catch “tactic not known”
+error:
+
+/--
+error: unsolved goals
+⊢ True
+-/
+#guard_msgs in
+example : True := by monotonicity
+
+-/
+
+open Lean.Internal.Order
+
+
+example : monotone (fun (f : Nat → Option Unit) => do {do f 1; f 2; f 3}) := by
+  repeat monotonicity
+
+-- The tactic only handels unary functions:
+
+/--
+error: Failed to prove monotonicity of:
+  fun x => x
+---
+error: Failed to prove monotonicity of:
+  fun x => x
+---
+error: Failed to prove monotonicity of:
+  fun x => x
+-/
+#guard_msgs in
+example : monotone (fun (f : Option Unit) => do {do f; f; f}) := by
+  monotonicity
+  · monotonicity
+  · monotonicity
+    monotonicity
+    · monotonicity
+    · monotonicity
+      monotonicity
